opaque WordAligned, and related cleanup
I generally just replaced multiplication by WORDSIZE with calls to
WordOffset or WordsToBytes, to establish alignment. remarkably few
reveals were needed, which makes me slightly suspicious, but in some
simple tests the opaque did appear to be working.

verified/ARMdef.dfy
@@ -1,26 +1,8 @@
 include "Maybe.dfy"
 include "Seq.dfy"
+include "types.s.dfy"
 include "bitvectors.s.dfy"
-include "alignment.s.dfy"
 include "words_and_bytes.s.dfy"
-
-//-----------------------------------------------------------------------------
-// Core types (for a 32-bit word-aligned machine)
-//-----------------------------------------------------------------------------
-const WORDSIZE:int := 4;
-predicate WordAligned(i:int) { i % WORDSIZE == 0 }
-function  WordsToBytes(w:int): int
-    ensures WordAligned(WordsToBytes(w))
-{ WORDSIZE * w }
-function  BytesToWords(b:int): int
-    requires WordAligned(b)
-{ b / WORDSIZE }
-
-function {:opaque} TruncateWord(x:int): word
-{ x % UINT32_LIM }
-
-type addr = x | isUInt32(x) && WordAligned(x)
-type shift_amount = s | 0 <= s < 32 // Some shifts allow s=32, but we'll be conservative for simplicity
 
 //-----------------------------------------------------------------------------
 // Microarchitectural State
@@ -43,6 +25,8 @@ datatype config = Config(cpsr:PSR, scr:SCR, ttbr0:TTBR,
 datatype PSR  = PSR(m:mode, f:bool, i:bool) // See B1.3.3
 datatype SCR  = SCRT(ns:world, irq:bool, fiq:bool) // See B4.1.129
 datatype TTBR = TTBR(ptbase:addr)      // See B4.1.154
+
+type shift_amount = s | 0 <= s < 32 // Some shifts allow s=32, but we'll be conservative for simplicity
 
 datatype Shift = LSLShift(amount_lsl:shift_amount)
                | LSRShift(amount_lsr:shift_amount)
@@ -653,16 +637,6 @@ predicate {:axiom} InterruptContinuationInvariant(s:state, r:state)
 // Model of page tables for userspace execution
 //-----------------------------------------------------------------------------
 
-const PAGESIZE:int := 0x1000;
-const PAGEBITS:int := 12;
-
-predicate {:opaque} PageAligned(addr:int)
-    ensures PageAligned(addr) ==> WordAligned(addr)
-{
-    lemma_PageAlignedImpliesWordAligned(addr);
-    addr % PAGESIZE == 0
-}
-
 function {:opaque} PageBase(addr:word): word
     ensures PageAligned(PageBase(addr))
 {
@@ -722,7 +696,7 @@ function AllPagesInTable(pt:AbsPTable): set<addr>
     requires WellformedAbsPTable(pt)
 {
     (set i, j | 0 <= i < |pt| && pt[i].Just? && 0 <= j < |pt[i].v|
-        && pt[i].v[j].Just? :: pt[i].v[j].v.phys + PhysBase())
+        && pt[i].v[j].Just? :: WordAlignedAdd(pt[i].v[j].v.phys, PhysBase()))
 }
 
 function WritablePagesInTable(pt:AbsPTable): set<addr>
@@ -731,13 +705,8 @@ function WritablePagesInTable(pt:AbsPTable): set<addr>
 {
     (set i, j | 0 <= i < |pt| && pt[i].Just? && 0 <= j < |pt[i].v|
         && pt[i].v[j].Just? && pt[i].v[j].v.write
-        :: pt[i].v[j].v.phys + PhysBase())
+        :: WordAlignedAdd(pt[i].v[j].v.phys, PhysBase()))
 }
-
-function WordOffset(a:addr, i:int): addr
-    requires isUInt32(a + WordsToBytes(i))
-    ensures WordAligned(WordOffset(a, i))
-{ a + WordsToBytes(i) }
 
 predicate ValidAbsL1PTable(m:memstate, vbase:int)
     requires ValidMemState(m)
@@ -1134,17 +1103,18 @@ predicate evalIns'(ins:ins, s:state, r:state)
             evalUpdate(s, rd, MemContents(s.m, OperandContents(s, base) +
                 OperandContents(s, ofs)), r)
         case LDR_global(rd, global, base, ofs) => 
-            evalUpdate(s, rd, GlobalWord(s.m, global, OperandContents(s, base)
-                + OperandContents(s, ofs) - AddressOfGlobal(global)), r)
+            evalUpdate(s, rd, GlobalWord(s.m, global,
+                WordAlignedSub(OperandContents(s, base) + OperandContents(s, ofs),
+                               AddressOfGlobal(global))), r)
         case LDR_reloc(rd, name) =>
             evalUpdate(s, rd, AddressOfGlobal(name), r)
         case STR(rd, base, ofs) => 
             evalMemUpdate(s, OperandContents(s, base) +
                 OperandContents(s, ofs), OperandContents(s, rd), r)
         case STR_global(rd, global, base, ofs) => 
-            evalGlobalUpdate(s, global, OperandContents(s, base)
-                + OperandContents(s, ofs) - AddressOfGlobal(global),
-                OperandContents(s, rd), r)
+            evalGlobalUpdate(s, global,
+                WordAlignedSub(OperandContents(s, base) + OperandContents(s, ofs),
+                               AddressOfGlobal(global)), OperandContents(s, rd), r)
         case MOV(dst, src) => evalUpdate(s, dst, OperandContents(s, src), r)
         case MOVW(dst, src) => evalUpdate(s, dst, OperandContents(s, src), r)
         case MOVT(dst, src) => evalUpdate(s, dst,
