verified/types.s.dfy
@@ -1,0 +1,89 @@
+//-----------------------------------------------------------------------------
+// Core types (for a 32-bit word-aligned machine)
+//-----------------------------------------------------------------------------
+
+const UINT32_LIM:int := 0x1_0000_0000;
+const WORDSIZE:int := 4;
+predicate isUInt32(i:int) { 0 <= i < UINT32_LIM }
+type word = x | isUInt32(x)
+
+predicate {:opaque} WordAligned(i:int) { i % WORDSIZE == 0 }
+
+type addr = x | (reveal WordAligned(); isUInt32(x) && WordAligned(x))
+
+function method WordsToBytes(w:int): int
+    ensures WordAligned(WordsToBytes(w))
+{ reveal WordAligned(); WORDSIZE * w }
+
+function method BytesToWords(b:int): int
+    requires WordAligned(b)
+{ reveal WordAligned(); b / WORDSIZE }
+
+function {:opaque} TruncateWord(x:int): word
+{ x % UINT32_LIM }
+
+function method WordOffset(a:addr, i:int): addr
+    requires isUInt32(a + WordsToBytes(i))
+    ensures WordAligned(WordOffset(a, i))
+{ a + WordsToBytes(i) }
+
+const PAGESIZE:int := 0x1000;
+const PAGEBITS:int := 12;
+
+predicate {:opaque} PageAligned(addr:int)
+    requires addr >= 0
+    ensures PageAligned(addr) ==> WordAligned(addr)
+{
+    if addr % PAGESIZE == 0
+    then lemma_PageAlignedImpliesWordAligned(addr); true
+    else false
+}
+
+lemma lemma_PageAlignedImplies1KAligned(addr:int)
+    requires addr >= 0 && addr % 0x1000 == 0
+    ensures addr % 0x400 == 0
+{ assert 0x1000 % 0x400 == 0; }
+
+lemma lemma_1KAlignedImpliesWordAligned(addr:int)
+    requires addr >= 0 && addr % 0x400 == 0
+    ensures WordAligned(addr)
+{
+    calc {
+        true;
+        addr % 0x400 == 0;
+        addr % 0x200 == 0;
+        addr % 0x100 == 0;
+        addr % 0x80 == 0;
+        addr % 0x40 == 0;
+        addr % 0x20 == 0;
+        addr % 0x10 == 0;
+        addr % 8 == 0;
+        addr % 4 == 0;
+        { reveal WordAligned(); }
+        WordAligned(addr);
+    }
+}
+
+lemma lemma_PageAlignedImpliesWordAligned(addr:int)
+    requires addr >= 0 && addr % 0x1000 == 0
+    ensures WordAligned(addr)
+{
+    lemma_PageAlignedImplies1KAligned(addr);
+    lemma_1KAlignedImpliesWordAligned(addr);
+}
+
+function WordAlignedAdd(x1:int, x2:int): int
+    requires WordAligned(x1) && WordAligned(x2)
+    ensures  WordAligned(WordAlignedAdd(x1, x2))
+{
+    reveal WordAligned();
+    x1 + x2
+}
+
+function WordAlignedSub(x1:int, x2:int): int
+    requires WordAligned(x1) && WordAligned(x2)
+    ensures  WordAligned(WordAlignedSub(x1, x2))
+{
+    reveal WordAligned();
+    x1 - x2
+}
